fstar/MLS.Crypto.Derived.fsti
@@ -8,6 +8,9 @@ open MLS.Result
 val available_ciphersuite_from_network: cipher_suite_nt -> result available_ciphersuite
 val available_ciphersuite_to_network: available_ciphersuite -> cipher_suite_nt
 
+val sign_with_label: #bytes:Type0 -> {|crypto_bytes bytes|} -> signature_key:sign_private_key bytes -> label:bytes -> content:bytes -> entropy:sign_nonce bytes -> result (sign_signature bytes)
+val verify_with_label: #bytes:Type0 -> {|crypto_bytes bytes|} -> verification_key:sign_public_key bytes -> label:bytes -> content:bytes -> signature:sign_signature bytes -> result bool
+
 val expand_with_label: #bytes:Type0 -> {|crypto_bytes bytes|} -> secret:bytes -> label:bytes -> context:bytes -> len:nat -> result (lbytes bytes len)
 val derive_secret: #bytes:Type0 -> {|crypto_bytes bytes|} -> secret:bytes -> label:bytes -> result (lbytes bytes (kdf_length #bytes))
 val make_hash_ref: #bytes:Type0 -> {|crypto_bytes bytes|} -> bytes -> result (lbytes bytes 16)
